completeness proof S5

src/language.lean
@@ -4,20 +4,21 @@ Released under the Apache License 2.0 (see "License");
 Author: Bruno Bentzen
 -/
 
-definition var : ℕ → Type := fin
-
 variable σ : nat
 
 /- language definition -/
 
 inductive form : Type
-| atom : var σ → form
+| atom : fin σ → form
 | bot : form
 | impl : form → form → form 
+| box : form → form
 
-notation `#` := form.atom
+prefix `#` := form.atom
 notation `⊥` := form.bot _
-notation `~` p := (form.impl p (form.bot _))
-notation p `⊃` q := (form.impl p q)
-notation p `&` q := (~ (p ⊃ ~q))
-notation p `∨` q := ~ (~p & ~q)
+infix `⊃` := form.impl
+notation `~`:40 p := form.impl p (form.bot _)
+notation p `&` q := ~(p ⊃ ~q)
+notation p `∨` q := ~(~p & ~q)
+prefix `◻`:80 := form.box
+prefix `◇`:80 := λ p, ~(◻ (~ p))
