src/context.lean
@@ -1,0 +1,15 @@
+/-
+Copyright (c) 2018 Bruno Bentzen. All rights reserved.
+Released under the Apache License 2.0 (see "License");
+Author: Bruno Bentzen
+-/
+
+import .language
+
+/- context -/ 
+
+@[reducible]
+def ctx (σ : nat) : Type := set (form σ)
+
+notation `·` := {}
+notation Γ ` ⸴ ` p := set.insert p Γ
