src/default.lean
@@ -4,5 +4,4 @@ Released under the Apache License 2.0 (see "License");
 Author: Bruno Bentzen
 -/
 
-import ..nat ..prime .language .context
-
+import data.set .language .context 
