src/mpl/default.lean
@@ -1,7 +1,0 @@
-/-
-Copyright (c) 2018 Bruno Bentzen. All rights reserved.
-Released under the Apache License 2.0 (see "License");
-Author: Bruno Bentzen
--/
-
-import ..nat ..prime .language .context
