src/s5/completeness.lean
@@ -1,0 +1,448 @@
+/-
+Copyright (c) 2018 Bruno Bentzen. All rights reserved.
+Released under the Apache License 2.0 (see "License");
+Author: Bruno Bentzen
+-/
+
+import .consistency ..encode
+
+open nat set classical
+
+local attribute [instance, priority 0] prop_decidable
+
+variables {σ : nat}
+
+/- maximal set of a context -/
+
+namespace ctx
+def is_max (Γ : ctx σ) := is_consist Γ ∧ ∀ p, p ∈ Γ ∨ (~p) ∈ Γ
+
+def insert_form (Γ : ctx σ) (p : form σ) : ctx σ :=
+if is_consist (Γ ⸴ p) then Γ ⸴ p else Γ ⸴ ~p
+
+def insert_code (Γ : ctx σ) (n : nat) : ctx σ :=
+match encodable.decode (form σ) n with
+| none := Γ
+| some p := insert_form Γ p
+end
+
+@[simp]
+def maxn (Γ : ctx σ) : nat → ctx σ
+| 0     := Γ
+| (n+1) := insert_code (maxn n) n
+
+@[simp]
+def max (Γ : ctx σ) : ctx σ := 
+⋃ n, maxn Γ n
+
+/- maximal extensions are extensions -/
+
+lemma subset_insert_code {Γ : ctx σ} (n) : 
+  Γ ⊆ insert_code Γ n :=
+begin
+  intros v hv,
+  unfold insert_code,
+  cases (encodable.decode (form σ) _); unfold insert_code insert_form,
+  { assumption },
+  { split_ifs; exact set.mem_insert_of_mem _ hv },
+end
+
+lemma subset_maxn {Γ : ctx σ} : 
+  ∀ n, Γ ⊆ maxn Γ n
+| 0        := by refl
+| (succ n) := subset.trans (subset_maxn n) (subset_insert_code _)
+
+lemma maxn_subset_max {Γ : ctx σ} (n) : 
+  maxn Γ n ⊆ max Γ :=
+subset_Union _ _
+
+lemma subset_max_self {Γ : ctx σ} :
+  Γ ⊆ max Γ :=
+maxn_subset_max 0
+
+lemma maxn_subset_succ {Γ : ctx σ} {n : nat} :
+  maxn Γ n ⊆ maxn Γ (n+1) :=
+subset_insert_code _
+
+lemma maxn_mono {Γ : ctx σ} {m n : nat} (h : n ≤ m) :
+  maxn Γ n ⊆ maxn Γ m :=
+by induction h; [refl, exact subset.trans h_ih (subset_insert_code _)]
+
+/- maximal extensions are maximal -/
+
+lemma insert_form_self {Γ : ctx σ} {p : form σ} : 
+  p ∈ insert_form Γ p ∨ (~p) ∈ insert_form Γ p :=
+begin
+  unfold insert_form, split_ifs,
+  { exact or.inl (mem_insert _ _) },
+  { exact or.inr (mem_insert _ _) },
+end
+
+lemma insert_code_self {Γ : ctx σ} (p : form σ) : 
+  p ∈ insert_code Γ (encodable.encode p) ∨ (~p) ∈ insert_code Γ (encodable.encode p) :=
+begin
+  unfold insert_code,
+  rw (encodable.encodek p),
+  apply insert_form_self,
+end
+
+lemma mem_or_mem_max {Γ : ctx σ} (p : form σ) : 
+  p ∈ max Γ ∨ (~p) ∈ max Γ :=
+begin
+  have := maxn_subset_max (encodable.encode p + 1),
+  exact (insert_code_self p).imp (@this _) (@this _),
+end
+
+/- maximal extensions preserves consistency -/
+
+lemma is_consist_insert_form {Γ : ctx σ} {p : form σ} 
+  (H : is_consist Γ) : is_consist (insert_form Γ p) :=
+begin
+  rw insert_form, split_ifs,
+  { exact h },
+  { exact inconsist_to_neg_consist H h },
+end
+
+lemma is_consist_insert_code {Γ : ctx σ} (n)
+  (H : is_consist Γ) : is_consist (insert_code Γ n) :=
+begin
+  rw insert_code, cases encodable.decode _ _,
+  { exact H },
+  { exact is_consist_insert_form H }
+end
+
+lemma is_consist_maxn {Γ : ctx σ} : 
+  ∀ n, is_consist Γ → is_consist (maxn Γ n)
+| 0 H := H
+| (n+1) H := is_consist_insert_code _ (is_consist_maxn _ H)
+
+lemma in_ext_ctx_max_set_is_in_ext_ctx_at {Γ : ctx σ} {p : form σ} :
+  (p ∈ max Γ) → ∃ n, p ∈ maxn Γ n :=
+mem_Union.1
+
+lemma ext_ctx_lvl {Γ : ctx σ} {p : form σ} :
+  (max Γ ⊢ₛ₅ p) → ∃ n, maxn Γ n ⊢ₛ₅ p :=
+begin
+  generalize eq : max Γ = Γ',
+  intro h, induction h; subst eq,
+    { cases in_ext_ctx_max_set_is_in_ext_ctx_at h_h,
+      constructor, 
+      apply prf.ax, 
+      assumption },
+
+    repeat {
+      constructor,
+      apply prf.pl1 <|> apply prf.pl2 <|> apply prf.pl3,
+      exact 0
+    },
+    
+    { cases h_ih_hpq rfl with n0 h_ext_pq, 
+      cases h_ih_hp rfl with n1 h_ext_p,
+        cases (prop_decidable (n0 ≤ n1)),
+            have hh: n1 ≤ n0 :=
+              begin
+                cases nat.le_total, 
+                assumption, 
+                contradiction 
+            end,
+          constructor,
+            apply prf.mp,
+            assumption,
+              apply prf.sub_weak,
+                exact h_ext_p,
+                apply maxn_mono,
+                assumption,
+          constructor,
+            apply prf.mp,
+              apply prf.sub_weak,
+                exact h_ext_pq,
+                apply maxn_mono,
+                assumption,
+              assumption },
+
+    { constructor,
+      apply prf.k,
+      exact 0 },
+
+    { constructor,
+      apply prf.t,
+      exact 0 },
+    
+    { constructor,
+      apply prf.s4,
+      exact 0 },
+    
+    { constructor,
+      apply prf.b,
+      exact 0 },
+    
+    { constructor,
+      apply prf.nec h_h,
+      exact 0 }
+end
+
+lemma is_consist_max {Γ : ctx σ} :
+  is_consist Γ → is_consist (max Γ) :=
+λ hc nc, let ⟨n, ht⟩ := ext_ctx_lvl nc in is_consist_maxn _ hc ht
+
+/- maximal consistent sets are closed under derivability -/
+
+lemma max_of_max {Γ : ctx σ} {p : form σ} (h : is_consist Γ) : is_max (max Γ) :=
+⟨ is_consist_max h , mem_or_mem_max⟩ 
+
+lemma mem_max_of_prf {Γ : ctx σ} {p : form σ} (h₁ : is_max Γ)
+  (h₂ : Γ ⊢ₛ₅ p) : p ∈ Γ :=
+(h₁.2 p).resolve_right $ λ hn,
+h₁.1 (prf.mp (prf.ax hn) h₂)
+
+end ctx
+
+/- the canonical model construction -/
+
+-- domain
+
+namespace canonical
+def domain (σ : nat) : set (wrld σ) := {w | ctx.is_max w}
+
+lemma mem_domain_max {w : wrld σ} :
+  w ∈ domain σ → ∀ p, (p ∈ w) ∨ ((~p) ∈ w) :=
+and.right
+
+lemma mem_domain_consist {w : wrld σ} :
+  w ∈ domain σ → is_consist w :=
+and.left
+
+lemma mem_domain {w : wrld σ}
+  (h : is_consist w) : ctx.max w ∈ domain σ :=
+⟨ctx.is_consist_max h, ctx.mem_or_mem_max⟩
+
+lemma mem_domain_of_prf {p : form σ} (w ∈ domain σ)
+  (h : w ⊢ₛ₅ p) : p ∈ w :=
+(mem_domain_max H p).resolve_right $
+λ hn, (mem_domain_consist H) (prf.mp (prf.ax hn) h)
+
+-- accessibility
+
+def unbox (w : wrld σ) : wrld σ := {p | (◻p) ∈ w}
+
+noncomputable def access : wrld σ → wrld σ → bool :=
+assume w v, if (unbox w ⊆ v) then tt else ff
+
+lemma subset_unbox_iff_access {w v : wrld σ} : access w v = tt ↔ unbox w ⊆ v :=
+by unfold access; simp 
+
+lemma mem_unbox_iff_mem_box {p : form σ} {w : wrld σ} :
+  p ∈ unbox w ↔ (◻p) ∈ w :=
+⟨ id, id ⟩ 
+
+lemma not_mem_unbox_of_mem_not_box {p : form σ} {w : wrld σ} (hc : w ∈ domain σ) :
+  (~◻p) ∈ w → p ∉ unbox w :=
+λ h np, (mem_domain_consist hc) (prf.mp (prf.ax h) (prf.ax (mem_unbox_iff_mem_box.1 np)))
+
+lemma mem_box_of_unbox_prf {p : form σ} {w : wrld σ} (H : w ∈ domain σ) :
+  (unbox w ⊢ₛ₅ p) → (◻p) ∈ w :=
+begin
+  generalize eq : unbox w = Γ',
+  intro h, induction h; subst eq,
+    { assumption },
+    repeat { apply ctx.mem_max_of_prf H,
+      apply prf.nec,
+      apply prf.pl1 <|> apply prf.pl2 <|> apply prf.pl3 },
+    { apply ctx.mem_max_of_prf H,
+      refine prf.mp (prf.ax _) (prf.ax (h_ih_hp rfl)),
+      exact (ctx.mem_max_of_prf H) (prf.mp prf.k (prf.ax (h_ih_hpq rfl))) },
+    { apply ctx.mem_max_of_prf H,
+      exact prf.nec prf.k },
+    { apply ctx.mem_max_of_prf H,
+      exact prf.nec prf.t },
+    { apply ctx.mem_max_of_prf H,
+      exact prf.nec prf.s4 },
+    { apply ctx.mem_max_of_prf H,
+      exact prf.nec prf.b },
+    { apply ctx.mem_max_of_prf H,
+      apply prf.nec (prf.nec h_h) }
+end
+
+lemma not_unbox_prf_of_not_box_mem {p : form σ} {w : wrld σ} (hw : w ∈ domain σ) :
+  (~◻p) ∈ w → (unbox w ⊬ₛ₅ p) :=
+by { intros h nhp, apply mem_domain_consist hw, apply prf.mp (prf.ax h) (prf.ax (mem_box_of_unbox_prf hw nhp)) }
+
+lemma consist_unbox_of_not_box_mem {p : form σ} {w : wrld σ} (hw : w ∈ domain σ) :
+  (~◻p) ∈ w → is_consist (unbox w ⸴ (~p)) :=
+λ hn, consist_not_of_not_prf (not_unbox_prf_of_not_box_mem hw hn)
+
+-- valuation
+
+noncomputable def val : fin σ → wrld σ → bool :=
+assume p w, if w ∈ domain σ ∧ (#p) ∈ w then tt else ff
+
+-- reflexivity
+
+lemma access.refl :
+  ∀ w ∈ domain σ, access w w = tt :=
+begin
+  intros w h, unfold access,
+  simp, intros p hp, cases mem_domain_max h p,
+  { assumption },
+  { exfalso, apply mem_domain_consist h,
+    apply prf.mp,
+    { apply prf.ax h_1 }, 
+    { apply prf.mp,
+      { apply prf.t },
+      { apply prf.ax,
+        apply mem_unbox_iff_mem_box.1,
+        assumption } } }
+end
+
+-- symmetry
+
+lemma access.symm : ∀ w ∈ domain σ, ∀ v ∈ domain σ, access w v = tt → access v w = tt :=
+begin
+  intros w hw v hv, unfold access,
+  simp, intros sw p hp,
+  apply mem_domain_of_prf _ hw,
+  apply prf.mp,
+    { apply prf.sub_weak, apply prf.contrap_b, simp },
+    { have h₁ : ∀ p, p ∉ v → p ∉ unbox w, from 
+      (λ p, (@not_imp_not _ _ (prop_decidable _)).2 (@sw _ ) ),
+      have h₂ : (◻~◻p) ∉ w, from 
+      begin
+        apply h₁,
+        intro h, apply mem_domain_consist hv,
+        apply prf.mp,
+        { apply prf.ax h }, 
+        { apply prf.ax, assumption }
+      end,
+      cases mem_domain_max hw (◻~◻p),
+      { contradiction },
+      { apply prf.ax, assumption } }
+end
+
+-- transitivity
+
+lemma access.trans : ∀ w ∈ domain σ, ∀ v ∈ domain σ, ∀ u ∈ domain σ,
+  access w v = tt → access v u = tt → access w u = tt :=
+begin
+  intros w hw v hv u hu, unfold access,
+  simp, intros sw sv p hp,
+  apply sv, apply mem_unbox_iff_mem_box.2,
+  apply sw, apply mem_unbox_iff_mem_box.2,
+  apply mem_domain_of_prf, assumption,
+  apply prf.mp,
+  { exact prf.s4 },
+  { apply prf.ax,
+    apply mem_unbox_iff_mem_box.1,
+    assumption }
+end
+
+noncomputable def model : @model σ :=
+begin
+  fapply model.mk,
+    apply domain,
+    apply access,
+    apply val,
+    apply access.refl,
+    apply access.symm,
+    apply access.trans
+end
+
+/- truth is membership in the canonical model -/
+
+lemma form_tt_iff_mem_wrld {p : form σ} : 
+  ∀ (w ∈ domain σ), (w ⊩⦃model⦄ p) = tt ↔ p ∈ w :=
+begin
+  induction p with v p q hp hq p hp,
+  { intros, unfold forces_form model val, simp,
+    apply iff.intro,
+    { intro h, exact h.right },
+    { intro h, split, repeat {assumption} } },
+  
+  { unfold forces_form, simp,
+    intros w wm h, apply mem_domain_consist wm (prf.ax h) },
+
+  { unfold forces_form, simp, intros v wm, 
+    apply iff.intro,
+    { intro h, cases h, 
+      { cases mem_domain_max wm p with h₁ h₂,
+        { refine ctx.mem_max_of_prf wm _, 
+          exact (prf.mp prf.pl1 (prf.ax ((hq _ wm).1 h))) },
+        { refine ctx.mem_max_of_prf wm _, 
+          apply prf.mp prf.contrap (prf.mp prf.pl1 (prf.ax h₂)) } },  
+      { cases mem_domain_max wm q with h₁ h₂,
+        { refine ctx.mem_max_of_prf wm _,
+          exact prf.mp prf.pl1 (prf.ax h₁) },
+        { refine ctx.mem_max_of_prf wm _,
+          refine prf.mp prf.contrap (prf.mp prf.pl1 _),
+          cases mem_domain_max wm p with hp₁ hp₂,
+          { exfalso, apply ff_eq_tt_eq_false,
+            transitivity, 
+            { exact h.symm },
+            { exact (hp _ wm).2 hp₁} },
+          { apply prf.ax hp₂ } } } },
+      { intro h,
+        cases mem_domain_max wm q with h₁ h₂,
+        { left, exact (hq _ wm).2 h₁ },
+        { cases mem_domain_max wm p with hp₁ hp₂,
+          { exfalso, apply mem_domain_consist wm,
+            exact prf.mp (prf.ax h₂) (prf.mp (prf.ax h) (prf.ax hp₁)) },
+          { right, apply eq_ff_of_not_eq_tt,
+            intro ptt, apply mem_domain_consist wm,
+            exact prf.mp (prf.ax hp₂) (prf.ax ((hp _ wm).1 ptt)) } } } },
+  
+  { unfold forces_form,
+    simp, intros w wm,
+    apply iff.intro,
+    { intro h,
+      cases mem_domain_max wm (◻p) with h₁ h₂,
+      { exact h₁ },
+        exfalso, apply ctx.is_consist_max (consist_unbox_of_not_box_mem wm h₂),
+        apply prf.mp,
+        { apply prf.ax (ctx.subset_max_self (mem_insert _ _)) },
+        { apply prf.ax, 
+          apply (hp _ (mem_domain (consist_unbox_of_not_box_mem wm h₂))).1,
+          apply h, apply mem_domain (consist_unbox_of_not_box_mem wm h₂), exact wm,
+          apply subset_unbox_iff_access.2,
+          intros p pm, apply ctx.subset_max_self,
+          apply mem_insert_of_mem _ pm } },
+      
+    { intro h,
+      intros w v, unfold model access, simp, 
+      intros wm' rwv, 
+      exact (hp _ v).2 (rwv (mem_unbox_iff_mem_box.2 h)) } }
+end
+
+lemma ctx_tt_of_mem_domain (Γ : ctx σ) (wm : Γ ∈ domain σ) : 
+  (Γ ⊩⦃model⦄ Γ) = tt :=
+mem_tt_to_ctx_tt Γ (λ p pm, (form_tt_iff_mem_wrld _ wm).2 pm)
+
+/- the completeness lemma -/
+
+theorem completeness {Γ : ctx σ} {p : form σ} : 
+  (Γ ⊨ₛ₅ p) → (Γ ⊢ₛ₅ p) :=
+begin
+  apply (@not_imp_not (Γ ⊢ₛ₅ p) (Γ ⊨ₛ₅ p) (prop_decidable _)).1,
+  intros nhp hp, cases hp,
+  have c : is_consist (Γ ⸴ ~p) := consist_not_of_not_prf nhp,
+  apply absurd,
+  fapply hp,
+    { exact model },
+    { exact ctx.max (Γ ⸴ ~p) },
+    { apply mem_domain c },
+
+    { apply cons_ctx_tt_to_ctx_tt,
+      apply ctx_tt_to_subctx_tt,
+      apply ctx_tt_of_mem_domain (ctx.max (Γ ⸴ ~p)),
+      apply mem_domain c,
+      apply ctx.subset_max_self },
+
+    { simp, apply eq_ff_of_not_eq_tt,
+      apply neg_tt_iff_ff.1, 
+      apply and.elim_right,
+      apply cons_ctx_tt_iff_and.1, 
+      apply ctx_tt_to_subctx_tt,
+      apply ctx_tt_of_mem_domain (ctx.max (Γ ⸴ ~p)),
+      apply mem_domain c,
+      apply ctx.subset_max_self },
+end
+
+end canonical
