src/s5/consistency.lean
@@ -1,0 +1,129 @@
+/-
+Copyright (c) 2018 Bruno Bentzen. All rights reserved.
+Released under the Apache License 2.0 (see "License");
+Author: Bruno Bentzen
+-/
+
+import .soundness 
+
+open prf classical
+
+variables {σ : nat}
+
+def is_consist (Γ : ctx σ) := Γ ⊬ₛ₅ ⊥
+
+lemma consist_not_of_not_prf {Γ : ctx σ} {p : form σ} :
+  (Γ ⊬ₛ₅ p) → is_consist (Γ ⸴ ~p) :=
+λ hnp hc, hnp (mp dne (deduction hc))
+
+lemma not_prf_of_consist_not {Γ : ctx σ} {p : form σ} :
+  is_consist (Γ ⸴ ~p) → (Γ ⊬ₛ₅ p) :=
+λ h c, h (conv_deduction (prf.mp prf.dni c))
+
+/- other notable properties of consistency -/
+
+lemma consist_of_not_prf {Γ : ctx σ} {p : form σ} : 
+  (Γ ⊬ₛ₅ p) → is_consist Γ :=
+λ nhp nc, nhp (ex_falso nc)
+
+lemma inconsist_to_neg_consist {Γ : ctx σ} {p : form σ} :
+  is_consist Γ → ¬is_consist (Γ ⸴ p) → is_consist (Γ ⸴ ~p) :=
+begin
+  intros c nc hp, apply c, apply mp,
+    apply deduction, apply by_contradiction nc,
+    apply mp dne, exact (deduction hp),
+end
+
+lemma inconsist_of_neg_to_consist {Γ : ctx σ} {p : form σ} :
+  is_consist Γ → ¬is_consist (Γ ⸴ ~p) → is_consist (Γ ⸴ p) :=
+begin
+  intros c nc hp, apply c, apply mp,
+  { apply deduction (by_contradiction nc) },
+  { exact deduction hp },
+end
+
+lemma consist_fst {Γ : ctx σ} {p : form σ} :
+  is_consist (Γ ⸴ p) → is_consist Γ :=
+λ hc hn,  hc (weak hn)
+
+/- consistent context extensions -/
+
+lemma consist_ext {Γ : ctx σ} {p : form σ} :
+  is_consist Γ  → (Γ ⊬ₛ₅ ~p) → is_consist (Γ ⸴ p) :=
+by intros c np hn; apply np (deduction hn)
+
+lemma inconsist_ext_to_inconsist {Γ : ctx σ} {p : form σ} :
+    ((¬is_consist (Γ ⸴ p)) ∧ ¬is_consist(Γ ⸴ ~p)) → ¬is_consist (Γ) :=
+begin
+  intros h nc, cases h,
+  have h₁ : ((Γ ⸴ p) ⊢ₛ₅ ⊥) := by_contradiction h_left,
+  have h₂ : ((Γ ⸴ ~p) ⊢ₛ₅ ⊥) := by_contradiction h_right,
+  apply nc, apply mp (deduction h₁),
+    apply mp dne (deduction h₂)
+end
+
+lemma consist_to_consist_ext {Γ : ctx σ} {p : form σ} :
+    is_consist (Γ) → (is_consist (Γ ⸴ p) ∨ is_consist (Γ ⸴ ~p)) :=
+begin
+  intro c, apply classical.by_contradiction, intro h, 
+  apply absurd c, apply inconsist_ext_to_inconsist,
+  apply (decidable.not_or_iff_and_not _ _).1, apply h,
+  repeat {apply (prop_decidable _)}
+end
+
+lemma pos_consist_mem {Γ : ctx σ} {p : form σ} :
+  p ∈ Γ → is_consist (Γ) → (~p) ∉ Γ :=
+λ hp hc hnp, hc (mp (ax hnp) (ax hp))
+
+lemma neg_consist_mem {Γ : ctx σ} {p : form σ} :
+  (~p) ∈ Γ → is_consist (Γ) → p ∉ Γ :=
+λ hnp hc hp, hc (mp (ax hnp) (ax hp))
+
+lemma pos_inconsist_ext {Γ : ctx σ} {p : form σ} (c : is_consist Γ) :
+  p ∈ Γ → ¬is_consist (Γ ⸴ p) → (~p) ∈ Γ :=
+begin
+  intros hp hn,
+  exfalso, apply c,
+  apply mp, apply deduction (by_contradiction hn),
+  apply ax hp
+end
+
+lemma neg_inconsist_ext {Γ : ctx σ} {p : form σ} (c : is_consist Γ) :
+  (~p) ∈ Γ → ¬is_consist (Γ ⸴ ~p) → p ∈ Γ :=
+begin
+  intros hp hn,
+  exfalso, apply c,
+  apply mp, apply deduction (by_contradiction hn),
+  apply ax hp
+end
+
+/- context extensions of subcontexts -/
+
+lemma sub_preserves_consist {Γ Δ : ctx σ} :
+  is_consist Γ  → is_consist Δ → Δ ⊆ Γ → is_consist (Γ ⊔ Δ) :=
+by intros c1 c2 s nc; apply c1; exact (subctx_contr s nc)
+
+lemma subctx_inherits_consist {Γ Δ : ctx σ} {p : form σ} :
+  is_consist Γ  → is_consist Δ → Γ ⊆ Δ → is_consist (Δ ⸴ p) → is_consist (Γ ⸴ p) :=
+by intros c1 c2 s c nc; apply c; apply conv_deduction; apply subctx_ax s (deduction nc)
+
+lemma inconsist_sub {Γ Δ : ctx σ} {p : form σ} (c : is_consist Γ) :
+  ¬is_consist (Δ ⸴ p) → Δ ⊆ Γ → ¬is_consist (Γ ⸴ p) :=
+begin
+  unfold is_consist, intros h s c, apply c,
+  apply subctx_ax, apply set.insert_subset_insert s,
+  apply classical.by_contradiction h
+end
+
+/- contradictions & interpretations -/
+
+lemma tt_to_const {Γ : ctx σ} {M : model} {w ∈ M.wrlds} :
+  (w ⊩⦃M⦄ Γ) = tt → is_consist Γ :=
+begin
+  intros h hin,
+  cases (sndnss hin),
+  apply bot_is_insatisf,
+  apply exists.intro,
+  refine (m M w _ h),
+  repeat {assumption},
+end
