src/s5/semantics/basic.lean
@@ -1,0 +1,45 @@
+/-
+Copyright (c) 2018 Bruno Bentzen. All rights reserved.
+Released under the Apache License 2.0 (see "License");
+Author: Bruno Bentzen
+-/
+
+import ..default
+
+open form classical
+
+@[reducible] def wrld (σ : nat) := ctx σ
+
+variable {σ : nat}
+
+/- Kripke models -/
+
+structure model := (wrlds : set (wrld σ)) (access : wrld σ → wrld σ → bool) (val : fin σ → wrld σ → bool)
+                   (refl : ∀ w ∈ wrlds, access w w = tt)
+                   (symm : ∀ w ∈ wrlds, ∀ v ∈ wrlds, access w v  = tt → access v w  = tt)
+                   (trans : ∀ w ∈ wrlds, ∀ v ∈ wrlds, ∀ u ∈ wrlds, access w v  = tt → access v u  = tt → access w u  = tt)
+
+local attribute [instance] prop_decidable
+
+noncomputable def forces_form (M : model) : form σ → wrld σ → bool
+|  (#p)   := λ w, M.val p w
+| (bot σ) := λ w, ff 
+| (p ⊃ q) := λ w, (bnot (forces_form p w)) || (forces_form q w) 
+|  (◻p)   := λ w,
+  if (∀ v ∈ M.wrlds, w ∈ M.wrlds → M.access w v = tt → forces_form p v = tt) then tt else ff
+
+/- Forcing -/
+
+notation w `⊩` `⦃` M `⦄ ` p := forces_form M p w
+
+/- Local logical consequence -/
+
+noncomputable def forces_ctx (M : model) (Γ : ctx σ) : wrld σ → bool :=
+assume w, if (∀ p, p ∈ Γ → forces_form M p w = tt) then tt else ff
+
+notation w `⊩` `⦃` M `⦄ ` p := forces_ctx M p w
+
+inductive sem_csq (Γ : ctx σ) (p : form σ) : Prop
+| is_true (m : ∀ (M : model) (w ∈ M.wrlds), ((w ⊩⦃M⦄ Γ) = tt) → (w ⊩⦃M⦄ p) = tt) : sem_csq
+
+notation Γ ` ⊨ₛ₅ ` p := sem_csq Γ p
