src/s5/soundness.lean
@@ -1,0 +1,72 @@
+/-
+Copyright (c) 2018 Bruno Bentzen. All rights reserved.
+Released under the Apache License 2.0 (see "License");
+Author: Bruno Bentzen
+-/
+
+import .syntax.lemmas .semantics.lemmas 
+
+variable {σ : nat}
+
+/- soundness -/
+
+theorem sndnss {Γ : ctx σ} {p : form σ} :
+  (Γ ⊢ₛ₅ p) → (Γ ⊨ₛ₅ p) :=
+begin
+  intro h,
+  induction h,
+  { apply sem_csq.is_true,
+    intros, apply ctx_tt_to_mem_tt,
+    repeat {assumption} },
+
+  { apply sem_csq.is_true,
+    intros M w wmem ctt,
+    apply is_true_pl1 },
+
+  { apply sem_csq.is_true,
+    intros M w wmem ctt,
+    apply is_true_pl2 },
+
+  { apply sem_csq.is_true,
+    intros M w wmem ctt,
+    apply is_true_pl3 },
+
+    { apply sem_csq.is_true,
+      induction h_ih_hpq,
+      induction h_ih_hp,
+      intros M w wmem ctt,
+      revert h_ih_hpq,
+      unfold forces_form, simp,
+      intro hpq,
+      cases (hpq M w wmem ctt),
+      { assumption },
+      { exfalso,
+        apply tt_eq_ff_eq_false,
+        rw eq.symm (h_ih_hp M w wmem ctt),
+        assumption } },
+      
+    { apply sem_csq.is_true,
+      intros M w wmem ctt, 
+      apply is_true_k },
+
+    { apply sem_csq.is_true,
+      intros M w wmem ctt,
+      apply is_true_t,
+      repeat {assumption} },
+
+    { apply sem_csq.is_true,
+      intros M w wmem ctt,
+      apply is_true_s4 },
+      
+    { apply sem_csq.is_true,
+      intros M w wmem ctt,
+      apply is_true_b },
+
+    { apply sem_csq.is_true,
+      intros M w wmem ctt,
+      unfold forces_form, simp,
+      induction h_ih,
+      intros v vmem wmem rwv,
+      apply h_ih, assumption,
+      apply empty_ctx_tt }
+end
