src/s5/syntax/basic.lean
@@ -1,0 +1,26 @@
+/-
+Copyright (c) 2018 Bruno Bentzen. All rights reserved.
+Released under the Apache License 2.0 (see "License");
+Author: Bruno Bentzen
+-/
+
+import ..default 
+
+variable {σ : nat}
+
+/- a general modal system -/
+
+inductive prf : ctx σ → form σ → Prop
+| ax {Γ} {p} (h : p ∈ Γ) : prf Γ p
+| pl1 {Γ} {p q} : prf Γ (p ⊃ (q ⊃ p))
+| pl2 {Γ} {p q r} : prf Γ ((p ⊃ (q ⊃ r)) ⊃ ((p ⊃ q) ⊃ (p ⊃ r)))
+| pl3 {Γ} {p q} :  prf Γ (((~p) ⊃ ~q) ⊃ (((~p) ⊃ q) ⊃ p))
+| mp {Γ} {p q} (hpq: prf Γ (p ⊃ q)) (hp : prf Γ p) : prf Γ q
+| k {Γ} {p q} : prf Γ (◻(p ⊃ q) ⊃ (◻p ⊃ ◻q))
+| t {Γ} {p} : prf Γ (◻p ⊃ p) 
+| s4 {Γ} {p} : prf Γ (◻p ⊃ ◻◻p) 
+| b {Γ} {p} : prf Γ (p ⊃ ◻◇p) 
+| nec {Γ} {p} (h : prf · p) : prf Γ (◻p)
+
+notation Γ ` ⊢ₛ₅ ` p := prf Γ p
+notation Γ ` ⊬ₛ₅ ` p := prf Γ p → false
