src/s5/syntax/lemmas.lean
@@ -1,0 +1,535 @@
+/-
+Copyright (c) 2018 Bruno Bentzen. All rights reserved.
+Released under the Apache License 2.0 (see "License");
+Author: Bruno Bentzen
+-/
+
+import .basic
+
+open prf
+
+variable {σ : nat}
+
+namespace prf
+
+/- identity implication -/
+
+lemma id {p : form σ} {Γ : ctx σ} :
+  Γ ⊢ₛ₅ p ⊃ p :=
+mp (mp (@pl2 σ Γ p (p ⊃ p) p) pl1) pl1
+
+/- deduction metatheorem -/
+
+theorem deduction {Γ : ctx σ} {p q : form σ} :
+  (Γ ⸴ p ⊢ₛ₅ q) → (Γ ⊢ₛ₅ p ⊃ q) :=
+begin
+  generalize eq : (Γ ⸴ p) = Γ',
+  intro h,
+  induction h; subst eq,
+  { repeat {cases h_h},
+    exact id,
+    { exact mp pl1  (ax h_h) } },
+  { exact mp pl1 pl1 },
+  { exact mp pl1 pl2 },
+  { exact mp pl1 pl3 },
+  { apply mp,
+    { exact (mp pl2 (h_ih_hpq rfl)) },
+    { exact h_ih_hp rfl } },
+  { exact mp pl1 k },
+  { exact mp pl1 t },
+  { exact mp pl1 s4 },
+  { exact mp pl1 b },
+  { exact mp pl1 (nec h_h) }
+end
+
+/- structural rules -/
+
+lemma sub_weak {Γ Δ : ctx σ} {p : form σ} :
+  (Δ ⊢ₛ₅ p) → (Δ ⊆ Γ) → (Γ ⊢ₛ₅ p) :=
+begin
+  intros h s,
+  induction h,
+  { apply ax, exact s h_h },
+  { exact pl1 },
+  { exact pl2 },
+  { exact pl3 },
+  { apply mp,
+    { exact h_ih_hpq s },
+    {exact h_ih_hp s} },
+  { exact k },
+  { exact t },
+  { exact s4 },
+  { exact b },
+  { exact nec h_h }
+end
+
+lemma weak {Γ : ctx σ} {p q : form σ} :
+  (Γ ⊢ₛ₅ p) → (Γ ⸴ q ⊢ₛ₅ p) :=
+begin
+  intro h,
+  induction h,
+  { apply ax,
+    exact (set.mem_insert_of_mem _ h_h) },
+  { exact pl1 },
+  { exact pl2 },
+  { exact pl3 },
+  { apply mp,
+    { exact h_ih_hpq },
+    { exact h_ih_hp } },
+  { exact k },
+  { exact t },
+  { exact s4 },
+  { exact b },
+  { exact nec h_h }
+end
+
+lemma contr {Γ : ctx σ} {p q : form σ} :
+  (Γ ⸴ p ⸴ p ⊢ₛ₅ q) → (Γ ⸴ p ⊢ₛ₅ q) :=
+begin
+  generalize eq : (Γ ⸴ p ⸴ p) = Γ',
+  intro h,
+  induction h; subst eq,
+  { apply ax,
+    cases set.eq_or_mem_of_mem_insert h_h,
+    { rw h, apply set.mem_insert},
+    { exact h } },
+  { exact pl1 },
+  { exact pl2 },
+  { exact pl3 },
+  { apply mp,
+    { exact h_ih_hpq rfl },
+    { exact h_ih_hp rfl } },
+  { exact k },
+  { exact t },
+  { exact s4 },
+  { exact b },
+  { exact nec h_h }
+end
+
+lemma exg {p q r : form σ} {Γ : ctx σ} :
+  (Γ ⸴ p ⸴ q ⊢ₛ₅ r) → (Γ ⸴ q ⸴ p ⊢ₛ₅ r) :=
+begin
+  generalize eq : (Γ ⸴ p ⸴ q) = Γ',
+  intro h,
+  induction h; subst eq,
+  { apply ax,
+    cases set.eq_or_mem_of_mem_insert h_h,
+    { rw h, apply set.mem_insert_of_mem _ _,
+      apply set.mem_insert _ _ },
+      { cases set.eq_or_mem_of_mem_insert h with h' h',
+        { rw h', apply set.mem_insert _ _ },
+        { apply set.mem_insert_of_mem _ _,
+          apply set.mem_insert_of_mem _ _, 
+          exact h' } } },
+  { exact pl1 },
+  { exact pl2 },
+  { exact pl3 },
+  { apply mp,
+    { exact h_ih_hpq rfl },
+    { exact h_ih_hp rfl } },
+  { exact k },
+  { exact t },
+  { exact s4 },
+  { exact b },
+  { exact nec h_h }
+end
+
+/- subcontext operations -/
+
+lemma subctx_ax {Γ Δ : ctx σ} {p : form σ} :
+   Δ ⊆ Γ → (Δ ⊢ₛ₅ p) → (Γ ⊢ₛ₅ p) :=
+begin
+  intros s h,
+  induction h,
+  { apply ax (s h_h) },
+  { exact pl1 },
+  { exact pl2 },
+  { exact pl3 },
+  { apply mp,
+    { exact h_ih_hpq s },
+    { exact h_ih_hp s } },
+  { exact k },
+  { exact t },
+  { exact s4 },
+  { exact b },
+  { exact nec h_h }
+end
+
+lemma subctx_contr {Γ Δ : ctx σ} {p : form σ}:
+   Δ ⊆ Γ → (Γ ∪ Δ ⊢ₛ₅ p) → (Γ ⊢ₛ₅ p) :=
+begin
+  generalize eq : Γ ∪ Δ = Γ',
+  intros s h,
+  induction h; subst eq,
+  { cases h_h,
+    { exact ax h_h },
+    { exact ax (s h_h) } },
+  { exact pl1 },
+  { exact pl2 },
+  { exact pl3 },
+  { apply mp,
+    { exact h_ih_hpq rfl },
+    { exact h_ih_hp rfl } },
+  { exact k },
+  { exact t },
+  { exact s4 },
+  { exact b },
+  { exact nec h_h }
+end
+
+/- right-hand side basic rules of inference -/
+
+lemma pr {Γ : ctx σ} {p : form σ} :
+  Γ ⸴ p ⊢ₛ₅ p :=
+by apply ax; apply or.intro_left; simp
+
+lemma pr1 {Γ : ctx σ} {p q : form σ} :
+  Γ ⸴ p ⸴ q ⊢ₛ₅ p :=
+by apply ax; apply or.intro_right; apply or.intro_left; simp
+
+lemma pr2 {Γ : ctx σ} {p q : form σ} :
+  Γ ⸴ p ⸴ q ⊢ₛ₅ q :=
+by apply ax; apply or.intro_left; simp
+
+lemma by_mp1 {Γ : ctx σ} {p q : form σ} :
+  Γ ⸴ p ⸴ p ⊃ q ⊢ₛ₅ q :=
+mp pr2 pr1
+
+lemma by_mp2 {Γ : ctx σ} {p q : form σ} :
+  Γ ⸴ p ⊃ q ⸴ p ⊢ₛ₅ q :=
+mp pr1 pr2
+
+lemma cut {Γ : ctx σ} {p q r : form σ} :
+  (Γ ⊢ₛ₅ p ⊃ q) → (Γ ⊢ₛ₅ q ⊃ r) → (Γ ⊢ₛ₅ p ⊃ r) :=
+λ hpq hqr, mp (mp pl2 (mp pl1 hqr)) hpq
+
+lemma conv_deduction {Γ : ctx σ} {p q : form σ} :
+  (Γ ⊢ₛ₅ p ⊃ q) → (Γ ⸴ p ⊢ₛ₅ q) :=
+λ h, mp (weak h) pr 
+
+/- left-hand side basic rules of inference -/
+
+lemma mp_in_ctx_left {Γ : ctx σ} {p q r : form σ} :
+  (Γ ⸴ p ⸴ q ⊢ₛ₅ r) → (Γ ⸴ p ⸴ p ⊃ q ⊢ₛ₅ r) :=
+begin
+  generalize eq : (Γ ⸴ p ⸴ q) = Γ',
+  intros h,
+  induction h; subst eq,
+  { cases h_h,
+    { rw h_h,
+      exact by_mp1 },
+    { cases h_h,
+      { rw h_h,
+        exact pr1 },
+      { apply ax,
+        apply set.mem_insert_of_mem _ _,
+        apply set.mem_insert_of_mem _ _, exact h_h } } },
+    { exact pl1 },
+    { exact pl2 },
+    { exact pl3 },
+    { apply mp,
+      { exact h_ih_hpq rfl },
+      { exact h_ih_hp rfl } },
+    { exact k },
+    { exact t },
+    { exact s4 },
+    { exact b },
+    { exact nec h_h }
+end
+
+lemma mp_in_ctx_right {Γ : ctx σ} {p q r : form σ} :
+  (Γ ⸴ p ⸴ p ⊃ q ⊢ₛ₅ r) → (Γ ⸴ p ⸴ q ⊢ₛ₅ r) :=
+begin
+  generalize eq : (Γ ⸴ p ⸴ p ⊃ q) = Γ',
+  intros h,
+  induction h; subst eq,
+  { cases h_h, 
+    { subst h_h,
+      exact mp pl1 pr },
+    { cases h_h,
+      { subst h_h, 
+        exact pr1 },
+      { exact weak (weak (ax h_h)) } } },    
+    { exact pl1 },
+    { exact pl2 },
+    { exact pl3 },
+    { apply mp,
+      { exact h_ih_hpq rfl },
+      { exact h_ih_hp rfl } },
+    { exact k },
+    { exact t },
+    { exact s4 },
+    { exact b },
+    { exact nec h_h }
+end
+
+/- basic lemmas -/
+
+lemma contrap {Γ : ctx σ} {p q : form σ} :
+  Γ ⊢ₛ₅ ((~q) ⊃ (~p)) ⊃ (p ⊃ q) :=
+deduction (deduction (mp (mp pl3 pr1) (mp pl1 pr2) ))
+
+lemma not_impl {Γ : ctx σ} {p q : form σ} : 
+  Γ ⊢ₛ₅ (p ⊃ q) ⊃ ((~q) ⊃ (~p)) :=
+begin
+  repeat { apply deduction },
+  apply mp,
+  { exact pr1 },
+    apply mp,
+    { apply ax,
+      apply set.mem_insert_of_mem,
+      apply set.mem_insert_of_mem,
+      apply set.mem_insert },
+    { exact pr2 }
+end
+
+lemma dne {p : form σ} {Γ : ctx σ} :
+  Γ ⊢ₛ₅ (~~p) ⊃ p :=
+have h : Γ ⊢ₛ₅ (~~p) ⊃ ((~p) ⊃ (~p)) := mp pl1 id,
+mp (mp pl2 (cut pl1 pl3)) h
+
+lemma dni {p : form σ} {Γ : ctx σ} :
+  Γ ⊢ₛ₅ p ⊃ (~~p) :=
+mp contrap dne 
+
+lemma lem {p : form σ} {Γ : ctx σ} :
+  Γ ⊢ₛ₅  p ∨ ~p :=
+mp dni (mp contrap dne)
+
+lemma not_impl_to_and {p q : form σ} {Γ : ctx σ} :
+  Γ ⊢ₛ₅ (~(p ⊃ q)) ⊃ (p & (~q)) :=
+begin
+  repeat {apply deduction},
+  apply (mp pr1),
+  { apply deduction,
+    apply mp,
+    { apply dne },
+    { exact (mp pr1 pr2) } },
+end
+
+lemma and_not_to_not_impl {p q : form σ} {Γ : ctx σ} :
+  Γ ⊢ₛ₅ (p & (~q)) ⊃ ~(p ⊃ q) :=
+begin
+  repeat {apply deduction},
+  apply mp,
+  { apply pr1 },
+  { apply cut,
+    { apply pr2 },
+    { apply dni } }
+end
+
+/- basic modal lemmas (K and B) -/
+
+lemma box_contrap {p q : form σ} :
+ · ⊢ₛ₅ (◻(p ⊃ q)) ⊃ (◻((~q) ⊃ ~p)) :=
+prf.mp (prf.k) (prf.nec prf.not_impl)
+
+lemma diamond_k {p q : form σ} :
+ · ⊢ₛ₅ (◻(p ⊃ q)) ⊃ ((◇p) ⊃ (◇q)) :=
+prf.deduction $ prf.mp prf.not_impl
+(prf.mp prf.k (prf.mp (prf.weak box_contrap) prf.pr ))
+
+lemma box_dne {p : form σ} :
+ · ⊢ₛ₅ (◻~~p) ⊃ (◻p) :=
+prf.mp (prf.k) (prf.nec (prf.dne))
+
+lemma box_dni {p : form σ} :
+ · ⊢ₛ₅ (◻p) ⊃ (◻~~p) :=
+prf.mp (prf.k) (prf.nec (prf.dni))
+
+lemma not_box_dni {p : form σ} :
+ · ⊢ₛ₅ (~◻p) ⊃ (~◻~~p) :=
+prf.mp prf.not_impl box_dne
+
+lemma not_box_dne {p : form σ} :
+ · ⊢ₛ₅ (~◻~~p) ⊃ (~◻p) :=
+prf.mp prf.not_impl box_dni
+
+lemma diamond_dne {p : form σ} :
+ · ⊢ₛ₅ (◇~~p) ⊃ (◇p) :=
+not_box_dne
+
+lemma diamond_dni {p : form σ} :
+ · ⊢ₛ₅ (◇p) ⊃ (◇~~p) :=
+not_box_dni
+
+lemma contrap_b {p : form σ} :
+ · ⊢ₛ₅ (◇◻p) ⊃ p :=
+begin
+  apply prf.cut,
+  show (· ⊢ₛ₅ (◇◻p) ⊃ (~◻~◻~~p)), 
+    from @prf.mp _ _ (◻(◻p ⊃ ◻(~~p))) _ diamond_k (prf.nec box_dni),
+  apply prf.cut,
+  show (· ⊢ₛ₅ (~◻~◻~~p) ⊃ ~~p),
+    from prf.mp prf.not_impl prf.b,
+  apply prf.dne
+end
+
+/- notable introduction rules -/
+
+lemma negintro {p q : form σ} {Γ : ctx σ} :
+  (Γ ⊢ₛ₅ p ⊃ q) → (Γ ⊢ₛ₅ p ⊃ ~q) → (Γ ⊢ₛ₅ ~p) :=
+have h : ∀ q, (Γ ⊢ₛ₅ p ⊃ q) → (Γ ⊢ₛ₅ (~~p) ⊃ q) := λ q h, cut dne h,
+  λ hp hnp, mp (mp pl3 (h (~q) hnp)) (h q hp)
+
+lemma ex_falso {Γ : ctx σ} {p : form σ} :
+  (Γ ⊢ₛ₅ ⊥) → (Γ ⊢ₛ₅ p) :=
+begin
+  intro h,
+  apply mp,
+  { exact dne },
+  { apply mp,
+    { exact pl1 },
+    { exact h } }
+end
+
+lemma ex_falso_and {Γ : ctx σ} {p q : form σ} :
+  Γ ⊢ₛ₅ (~p) ⊃ (p ⊃ q) :=
+begin
+  repeat {apply deduction},
+  apply ex_falso,
+  exact (mp pr1 pr2)
+end
+
+lemma ex_falso_pos {Γ : ctx σ} {p q : form σ} :
+  Γ ⊢ₛ₅ p ⊃ ((~p) ⊃ q) :=
+begin
+  repeat {apply deduction},
+  apply mp,
+  { apply mp,
+    { apply ex_falso_and },
+    { exact pr2 } },
+  { exact pr1 },
+end
+
+lemma contr_conseq {Γ : ctx σ} {p r : form σ} :
+  Γ ⊢ₛ₅ (p ⊃ r) ⊃ (((~p) ⊃ r) ⊃ r) :=
+begin
+  repeat {apply deduction},
+  apply mp,
+  { apply mp,
+    { apply pl3, exact p },
+    { apply mp,
+      { apply not_impl },
+      { exact pr1 } } },
+  { apply cut,
+    { apply mp,
+      { apply not_impl,
+        exact (~p) },
+      { apply pr2 } },
+        apply dne }
+end
+
+lemma impl_weak {p q r : form σ} {Γ : ctx σ} (h : (Γ ⸴ r ⊢ₛ₅ p) → (Γ ⊢ₛ₅ p)) :
+  ((Γ ⊢ₛ₅ p) → (Γ ⊢ₛ₅ q)) → ((Γ ⸴ r ⊢ₛ₅ p) → (Γ ⸴ r ⊢ₛ₅ q)) :=
+λ hpq hp, weak (hpq (h hp))
+
+lemma and_intro {Γ : ctx σ} {p q : form σ} :
+  (Γ ⊢ₛ₅ p) → (Γ ⊢ₛ₅ q) → (Γ ⊢ₛ₅ (p & q)) :=
+begin
+  intros hp hq,
+  apply deduction,
+  apply mp,
+    apply mp,
+    { apply pr },
+    repeat { apply weak, assumption }
+end
+
+
+lemma and_elim_left {p q : form σ} {Γ : ctx σ} :
+  (Γ ⸴ (p & q) ⊢ₛ₅ p) :=
+begin
+  apply mp,
+  { apply dne },
+  { apply mp,
+    { apply mp,
+      { apply pl2, exact (p ⊃ (q ⊃ ⊥)) },
+      { apply mp,
+        { apply pl1 },
+        { exact pr } } },
+    { exact ex_falso_and } }
+end
+
+lemma and_elim_right {p q : form σ} {Γ : ctx σ} :
+  (Γ ⸴ (p & q) ⊢ₛ₅ q) :=
+begin
+  apply mp,
+  { apply dne },
+  { apply mp,
+    { apply mp,
+      { apply pl2, exact (p ⊃ (q ⊃ ⊥)) },
+      { apply mp,
+        { apply pl1 },
+        { exact pr } } },
+    repeat {apply deduction},
+    apply mp,
+    { apply ax,
+      apply set.mem_insert_of_mem,
+      apply set.mem_insert_of_mem,
+      apply set.mem_insert },
+    { exact pr2 } }
+end
+
+lemma or_intro_left {Γ : ctx σ} {p q r : form σ} :
+  (Γ ⊢ₛ₅ p) → (Γ ⊢ₛ₅ (p ∨ q)) :=
+begin
+  intros hp, simp,
+  apply mp,
+  { apply dni },
+  { apply deduction,
+    { apply mp,
+      { apply mp,
+        { apply ex_falso_and },
+        { exact pr } },
+      { apply weak, assumption } } }
+end
+
+lemma or_intro_right {Γ : ctx σ} {p q r : form σ} :
+  (Γ ⊢ₛ₅ q) → (Γ ⊢ₛ₅ (p ∨ q)) :=
+begin
+  intros hp, simp,
+  apply mp,
+  { apply dni },
+  { apply deduction,
+    { apply mp,
+      { apply dni },
+      {apply weak, assumption } } }
+end
+
+lemma or_elim {Γ : ctx σ} {p q r : form σ} :
+  (Γ ⊢ₛ₅ (p ∨ q)) → (Γ ⊢ₛ₅ p ⊃ r) → (Γ ⊢ₛ₅ q ⊃ r) → (Γ ⊢ₛ₅ r) :=
+begin
+  intros hpq hpr hqr,
+  apply mp,
+    { apply mp,
+      { apply contr_conseq, exact p },
+      { assumption } },
+    { apply cut,
+      { apply mp,
+        { apply dne },
+        { assumption } },
+      { apply cut,
+        exact dne,
+        assumption } }
+end
+
+lemma detach_pos {Γ : ctx σ} {p q : form σ} :
+  (Γ ⸴ p ⊢ₛ₅ q) → (Γ ⸴ ~p ⊢ₛ₅ q) → (Γ ⊢ₛ₅ q) :=
+begin
+  intros hpq hnpq,
+  apply or_elim,
+  { apply lem },
+  repeat {apply deduction, assumption}
+end
+
+lemma detach_neg {Γ : ctx σ} {p q : form σ} :
+  (Γ ⸴ ~p ⊢ₛ₅ q) → (Γ ⸴ p ⊢ₛ₅ q) → (Γ ⊢ₛ₅ q) :=
+begin
+  intros hpq hnpq,
+  apply or_elim,
+  { apply lem },
+  { apply deduction, exact hnpq },
+  { apply deduction, assumption }
+end
+
+end prf
